cedar-lean/Cedar/Thm/TPE/BatchedWellTyped.lean
@@ -1,0 +1,36 @@
+import Cedar.TPE
+import Cedar.Thm.TPE.Input
+import Cedar.Thm.TPE.PreservesTypeOf
+import Cedar.Thm.TPE.WellTypedCases
+import Cedar.Thm.Validation.WellTyped.ResidualDefinition
+import Cedar.Thm.Data.List
+import Cedar.Thm.Data.Map
+
+/-!
+This file contains theorems about partial evaluation preserving well-typedness of residuals.
+-/
+
+namespace Cedar.Thm
+
+open Cedar.Thm
+open Cedar.Data
+open Cedar.Spec
+open Cedar.Validation
+open Cedar.TPE
+
+
+theorem batched_eval_loop_preserves_well_typed
+  (loader) (store) (i)
+  {env : TypeEnv}
+  {res : Residual}
+  {req : Request}
+  {es : Entities}
+  {pes : PartialEntities} :
+  InstanceOfWellFormedEnvironment req es env →
+  RequestAndEntitiesRefine req es (req.asPartialRequest) pes →
+  Residual.WellTyped env res →
+  Residual.WellTyped env (batchedEvalLoop res req loader store i)
+:= by
+  sorry
+
+end Cedar.Thm
